Implement and almost prove read_bytes

src/SlowByteFile.v
@@ -121,6 +121,27 @@ Module SLOWBYTEFILE.
      fsxp.(FSXPLog) fsxp.(FSXPInode) inum ($ off) mscs;
      rx ^(mscs, b).
 
+  Definition read_bytes T fsxp inum (off:nat) len mscs rx : prog T :=
+    let^ (mscs, databytes) <- For i < len
+      Ghost [ m mbase F Fm A f flist bytes ]
+      Loopvar [ mscs l ]
+      Continuation lrx
+      Invariant
+          LOG.rep fsxp.(FSXPLog) F (ActiveTxn mbase m) mscs *
+          [[ (Fm * BFILE.rep fsxp.(FSXPBlockAlloc) fsxp.(FSXPInode) flist)%pred (list2mem m) ]] *
+          [[ (A * #inum |-> f)%pred (list2nmem flist) ]] *
+          [[ rep bytes f ]] *
+          [[ l = firstn #i (skipn off bytes) ]]
+     OnCrash
+      exists m',
+        LOG.rep fsxp.(FSXPLog) F (ActiveTxn mbase m') mscs
+     Begin
+      let^ (mscs, b) <- BFileRec.bf_get byte_type items_per_valu itemsz_ok
+        fsxp.(FSXPLog) fsxp.(FSXPInode) inum ($ (off + #i)) mscs;
+      lrx ^(mscs, l ++ [b])
+    Rof ^(mscs, nil);
+    rx ^(mscs, databytes).
+
   Lemma bound_helper : forall a b,
     # (natToWord addrlen b) = b -> a <= b -> a <= # (natToWord addrlen b).
   Proof.
@@ -255,6 +276,122 @@ Module SLOWBYTEFILE.
     reflexivity.
     apply Nat.lt_le_incl. eassumption.
   Qed.
+
+  Lemma app_prefix_eq : forall T (l: list T) x y,
+    x = y -> l ++ [x] = l ++ [y].
+  Proof.
+    intros.
+    subst.
+    reflexivity.
+  Qed.
+
+  Lemma selN_skip_first : forall T (l:list T) n m p def,
+    n + m < p ->
+    selN l (n + m) def = selN (skipn n (firstn p l)) m def.
+   Proof.
+    intros.
+    rewrite skipn_selN.
+    rewrite selN_firstn.
+    reflexivity.
+    assumption.
+  Qed.
+
+  Theorem read_bytes_ok: forall fsxp inum off len mscs,
+  {< m mbase F Fx Fm A flist f bytes v,
+  PRE LOG.rep (FSXPLog fsxp) F (ActiveTxn mbase m) mscs *
+      [[ (Fm * BFILE.rep (FSXPBlockAlloc fsxp) (FSXPInode fsxp) flist)%pred (list2mem m) ]] *
+      [[ (A * #inum |-> f)%pred (list2nmem flist) ]] *
+      [[ rep bytes f ]] *
+      [[ length v = #len ]] *
+      [[ (Fx * arrayN off v)%pred (list2nmem bytes) ]] *
+      [[ off + #len <= length bytes ]]
+   POST RET:^(mscs, databytes)
+      LOG.rep (FSXPLog fsxp) F (ActiveTxn mbase m) mscs *
+      [[ databytes = v ]]
+   CRASH LOG.would_recover_old (FSXPLog fsxp) F mbase
+   >} read_bytes fsxp inum off len mscs.
+   Proof.
+    unfold read_bytes, rep, bytes_rep.
+
+    step. (* enter loop *)
+    exists allbytes.
+    split;  auto.
+
+    step. (* bf_get *)
+    (* we assert and prove this lemma first because it is used twice *)
+    assert (Hoffm1: off + #(m1) < length allbytes0).
+      (* without the bounds checking, this proof goes:
+      m1 < off -> m1 < len
+      -> off + m1 < off + len
+      off + len < min( f.isize, length allbytes ) (firstn_length)
+      length allbytes0 >= f.isize (from roundup_ok)
+      -> off + len < f.isize <= length allbytes0
+      -> off + m1 < length allbytes0 *)
+    apply le_trans with (off + #(len)).
+    apply plus_lt_compat_l. apply wlt_lt. assumption.
+    rewrite firstn_length in H4.
+    apply Nat.min_glb_l in H4.
+    apply le_trans with (# (INODE.ISize (BFILE.BFAttr f))). assumption.
+    rewrite <- H22.
+    apply roundup_ok.
+    erewrite wordToNat_natToWord_bound.
+    apply Hoffm1.
+    instantiate (bound := $ (length allbytes0)).
+    rewrite H20.
+    omega.
+
+    step.
+    exists allbytes; split; auto.
+    subst.
+      (* same charade as above *)
+      assert (Hoffm1: off + #(m1) < #(INODE.ISize (BFILE.BFAttr f))).
+      rewrite firstn_length in H4.
+      apply Nat.min_glb_l in H4.
+      apply le_trans with (off + #(len)).
+      apply plus_lt_compat_l. apply wlt_lt. assumption.
+      assumption.
+    replace (# (m1 ^+ $ (1))) with (# (m1) + 1).
+    erewrite firstn_plusone_selN.
+    apply app_prefix_eq.
+    rewrite <- H16.
+    unfold sel.
+
+    erewrite wordToNat_natToWord_bound.
+    apply selN_skip_first.
+    apply Hoffm1.
+    apply Nat.lt_le_incl.
+    eassumption.
+    rewrite skipn_length.
+    apply Nat.lt_add_lt_sub_r.
+    rewrite plus_comm.
+    rewrite H18.
+    apply Hoffm1.
+    rewrite H18.
+    omega.
+    (* need to convert ^+ $(1) to +1 using bounds *)
+      rewrite wplus_alt.
+      unfold wplusN, wordBinN.
+      simpl.
+      erewrite wordToNat_natToWord_bound.
+      reflexivity.
+      (* same as H3, after some massaging *)
+      apply wlt_lt in H3.
+      unfold lt in H3.
+      instantiate (bound := len).
+      replace (# (m1) + 1) with (S # (m1)) by omega.
+      eassumption.
+    step.
+
+    (* no lemma available, but consequence of:
+    arrayN off allbytes ->
+    off < length allbytes ->
+    len = length v9 ->
+    firstn len (skipn off allbytes) = v9
+    (with many details left out) *)
+    admit.
+
+    apply LOG.activetxn_would_recover_old.
+  Admitted.
 
 
   Theorem update_bytes_ok: forall fsxp inum off newdata mscs,
